impl_map_group_filter

src/cddl/pulse/CDDL.Pulse.MapGroup.fst
@@ -45,10 +45,202 @@ let rec match_linked_list
   (l: list (cbor & cbor))
 : Tot slprop
   (decreases l)
-= match ll, l with
-  | _, [] -> pure (None? ll)
-  | Some c, a :: q -> match_linked_list_cons l0 c a q (match_linked_list l0)
-  | _ -> pure False
+= match l with
+  | [] -> pure (None? ll)
+  | a :: q ->
+    begin match ll with
+    | Some c -> match_linked_list_cons l0 c a q (match_linked_list l0)
+    | _ -> pure False
+    end
+
+```pulse
+ghost
+fn match_linked_list_is_nil
+  (ll: linked_list)
+  (#l0: (list (cbor & cbor)))
+  (#l: (list (cbor & cbor)))
+requires
+  match_linked_list l0 ll l
+ensures
+  match_linked_list l0 ll l **
+  pure (None? ll == Nil? l)
+{
+  match l {
+    Nil -> {
+      unfold (match_linked_list l0 ll []);
+      fold (match_linked_list l0 ll []);
+    }
+    Cons a q -> {
+      match ll {
+        None -> {
+          unfold (match_linked_list l0 None (a :: q));
+          fold (match_linked_list l0 None (a :: q))
+        }
+        Some c -> { () }
+      }
+    }
+  }
+}
+```
+
+```pulse
+ghost
+fn match_linked_list_cons_elim
+  (ll: linked_list)
+  (c: linked_list_cell)
+  (#l0: (list (cbor & cbor)))
+  (#l: (list (cbor & cbor)))
+requires
+  match_linked_list l0 ll l **
+  pure (Cons? l /\
+    ll == Some c
+  )
+returns res: squash (Cons? l)
+ensures exists* ll' .
+  R.pts_to c.tail ll' **
+  match_linked_list l0 ll' (List.Tot.tl l) **
+  Trade.trade
+    (R.pts_to c.tail ll' **
+      match_linked_list l0 ll' (List.Tot.tl l))
+    (match_linked_list l0 ll l) **
+  pure (
+    let i = U64.v (c.value) in
+    i < List.Tot.length l0 /\
+    List.Tot.index l0 i == List.Tot.hd l)
+{
+  match_linked_list_is_nil ll;
+  let a = List.Tot.hd l;
+  let q = List.Tot.tl l;
+  unfold (match_linked_list l0 (Some c) (a :: q));
+  unfold (match_linked_list_cons l0 c a q (match_linked_list l0));
+  with ll' . assert (R.pts_to c.tail ll' ** match_linked_list l0 ll' q);
+  ghost fn aux ()
+    requires emp ** (R.pts_to c.tail ll' ** match_linked_list l0 ll' q)
+    ensures match_linked_list l0 ll l
+  {
+    fold (match_linked_list_cons l0 c a q (match_linked_list l0));
+    fold (match_linked_list l0 (Some c) (a :: q));
+  };
+  Trade.intro _ _ _ aux;
+  ()
+}
+```
+
+let rec list_index_map
+  (#t1 #t2: Type)
+  (f: (t1 -> t2))
+  (l: list t1)
+  (i: nat)
+: Lemma
+  (requires (i < List.Tot.length l))
+  (ensures (
+    let l' = List.Tot.map f l in
+    i < List.Tot.length l' /\
+    List.Tot.index l' i == f (List.Tot.index l i)
+  ))
+  [SMTPat (List.Tot.index (List.Tot.map f l) i)]
+= if i = 0
+  then ()
+  else list_index_map f (List.Tot.tl l) (i - 1)
+
+let rec list_no_repeats_index_inj'
+  (#t: Type)
+  (l: list t)
+  (i1 i2: nat)
+: Lemma
+  (requires (i1 <= i2 /\ i2 < List.Tot.length l /\
+    List.Tot.no_repeats_p l /\
+    List.Tot.index l i1 == List.Tot.index l i2
+  ))
+  (ensures (
+    i1 == i2
+  ))
+  (decreases l)
+= if i1 = 0
+  then ()
+  else list_no_repeats_index_inj' (List.Tot.tl l) (i1 - 1) (i2 - 1)
+
+let list_no_repeats_index_inj
+  (#t: Type)
+  (l: list t)
+  (i1 i2: nat)
+: Lemma
+  (requires (i1 < List.Tot.length l /\
+    i2 < List.Tot.length l /\
+    List.Tot.no_repeats_p l    
+  ))
+  (ensures (
+    (i1 == i2 <==> List.Tot.index l i1 == List.Tot.index l i2)
+  ))
+= if (i1 <= i2)
+  then Classical.move_requires (list_no_repeats_index_inj' l i1) i2
+  else Classical.move_requires (list_no_repeats_index_inj' l i2) i1
+
+inline_for_extraction
+```pulse
+fn match_linked_list_mem
+  (ll: linked_list)
+  (x: U64.t)
+  (#l0: Ghost.erased (list (cbor & cbor)))
+  (#l: Ghost.erased (list (cbor & cbor)))
+requires
+  match_linked_list l0 ll l **
+  pure (
+    List.Tot.no_repeats_p (List.Tot.map fst l0) /\
+    U64.v x < List.Tot.length l0
+  )
+returns res: bool
+ensures
+  match_linked_list l0 ll l **
+  pure (U64.v x < List.Tot.length l0 /\
+    res == Some? (List.Tot.assoc (fst (List.Tot.index l0 (U64.v x))) l)
+  )
+{
+  let mut pll = ll;
+  let mut pres = false;
+  Trade.refl (match_linked_list l0 ll l);
+  while (
+    let res = !pres;
+    if (res) {
+      false
+    } else {
+      let ll1 = !pll;
+      match_linked_list_is_nil ll1;
+      Some? ll1
+    }
+  )
+  invariant b . exists* ll1 l1 res .
+    R.pts_to pll ll1 **
+    match_linked_list l0 ll1 l1 **
+    Trade.trade
+      (match_linked_list l0 ll1 l1)
+      (match_linked_list l0 ll l) **
+    R.pts_to pres res **
+    pure (
+      Some? (List.Tot.assoc (fst (List.Tot.index l0 (U64.v x))) l) == (res || Some? (List.Tot.assoc (fst (List.Tot.index l0 (U64.v x))) l1)) /\
+      b == (Cons? l1 && not res)
+    )
+  {
+    let ll1 = !pll;
+    match_linked_list_is_nil ll1;
+    let c = Some?.v ll1;
+    match_linked_list_cons_elim ll1 c;
+    let i = c.value;
+    list_no_repeats_index_inj (List.Tot.map fst l0) (U64.v x) (U64.v i);
+    if (x = i) {
+      Trade.elim _ (match_linked_list l0 ll1 _);
+      pres := true;
+    } else {
+      Trade.trans _ _ (match_linked_list l0 ll l);
+      let ll2 = ! c.tail;
+      Trade.elim_hyp_l _ _ _;
+      pll := ll2;
+    }
+  };
+  Trade.elim _ _;
+  !pres
+}
+```
 
 let list_not_defined_at
   (#t: eqtype)
@@ -72,8 +264,10 @@ let impl_map_group_for_excluded_post
 =
   match res, apply_map_group_det g (cbor_map_filter (list_not_defined_at vexcluded) m) with
               | MGOK, MapGroupDet _ rem -> rem == cbor_map_empty
-              | MGFail, MapGroupFail -> True
               | MGCutFail, MapGroupCutFail -> True
+              | _, MapGroupNonDet -> False
+              | MGFail, MapGroupDet _ rem -> ~ (rem == cbor_map_empty)
+              | MGFail, MapGroupFail -> True
               | _ -> False
 
 inline_for_extraction noextract [@@noextract_to "krml"]
@@ -170,6 +364,260 @@ fn impl_map_group_concat
   (_: unit)
 {
   ig1 i #p #l m g2 (ig2 i #p #l m) pexcluded #lexcluded #vexcluded ()
+}
+```
+
+module U = CBOR.Spec.Util
+
+let cbor_map_filter_true_eq : squash (map_group_filter (U.truep) == map_group_nop)
+= assert (forall f . cbor_map_filter (U.notp U.truep) f `cbor_map_equal` cbor_map_empty);
+  apply_map_group_det_map_group_equiv (map_group_filter (U.truep)) map_group_nop
+
+inline_for_extraction noextract [@@noextract_to "krml"]
+let impl_map_entry_cond
+  (#t: Type)
+  (vmatch2: perm -> t -> cbor & cbor -> slprop)
+  (f: ((cbor & cbor) -> bool))
+=
+  (x: t) ->
+  (#p: perm) ->
+  (#v: Ghost.erased (cbor & cbor)) ->
+  stt bool
+    (vmatch2 p x v)
+    (fun res -> vmatch2 p x v ** pure (res == f v))
+
+inline_for_extraction noextract [@@noextract_to "krml"]
+```pulse
+fn impl_map_entry_cond_true
+  (#t: Type0)
+  (vmatch2: perm -> t -> cbor & cbor -> slprop)
+: impl_map_entry_cond u#0 #t vmatch2 U.truep
+= (x: _)
+  (#p: _)
+  (#v: _)
+{
+  true
+}
+```
+
+inline_for_extraction noextract [@@noextract_to "krml"]
+```pulse
+fn impl_map_entry_cond_not
+  (#t: Type0)
+  (#vmatch2: perm -> t -> cbor & cbor -> slprop)
+  (#f: Ghost.erased ((cbor & cbor) -> bool))
+  (impf: impl_map_entry_cond vmatch2 f)
+: impl_map_entry_cond u#0 #t vmatch2 (U.notp f)
+= (x: _)
+  (#p: _)
+  (#v: _)
+{
+  let nres = impf x;
+  not nres
+}
+```
+
+inline_for_extraction noextract [@@noextract_to "krml"]
+```pulse
+fn impl_map_entry_cond_and
+  (#t: Type0)
+  (#vmatch2: perm -> t -> cbor & cbor -> slprop)
+  (#f1: Ghost.erased ((cbor & cbor) -> bool))
+  (impf1: impl_map_entry_cond vmatch2 f1)
+  (#f2: Ghost.erased ((cbor & cbor) -> bool))
+  (impf2: impl_map_entry_cond vmatch2 f2)
+: impl_map_entry_cond u#0 #t vmatch2 (U.andp f1 f2)
+= (x: _)
+  (#p: _)
+  (#v: _)
+{
+  let res1 = impf1 x;
+  if (res1) {
+    impf2 x
+  } else {
+    false
+  }
+}
+```
+
+inline_for_extraction noextract [@@noextract_to "krml"]
+```pulse
+fn impl_map_entry_cond_or
+  (#t: Type0)
+  (#vmatch2: perm -> t -> cbor & cbor -> slprop)
+  (#f1: Ghost.erased ((cbor & cbor) -> bool))
+  (impf1: impl_map_entry_cond vmatch2 f1)
+  (#f2: Ghost.erased ((cbor & cbor) -> bool))
+  (impf2: impl_map_entry_cond vmatch2 f2)
+: impl_map_entry_cond u#0 #t vmatch2 (orp f1 f2)
+= (x: _)
+  (#p: _)
+  (#v: _)
+{
+  let res1 = impf1 x;
+  if (res1) {
+    true
+  } else {
+    impf2 x
+  }
+}
+```
+
+let list_nil_forall_not_memP
+  (#t: Type)
+  (l: list t)
+: Lemma
+  (Nil? l <==> forall x . ~ (List.Tot.memP x l))
+= ()
+
+module GR = Pulse.Lib.GhostReference
+
+let rec list_index_append_cons
+  (#t: Type)
+  (l1: list t)
+  (x: t)
+  (l2: list t)
+: Lemma
+  (ensures (let i = List.Tot.length l1 in
+    let l = List.Tot.append l1 (x :: l2) in
+    i < List.Tot.length l /\
+    List.Tot.index l i == x
+  ))
+  (decreases l1)
+= match l1 with
+  | [] -> ()
+  | _ :: q -> list_index_append_cons q x l2
+
+let list_filter_cons_intro
+  (#t: Type)
+  (f: t -> bool)
+  (a: t)
+  (q: list t)
+: Lemma
+  (requires (f a))
+  (ensures (Cons? (List.Tot.filter f (a :: q))))
+= ()
+
+inline_for_extraction noextract [@@noextract_to "krml"]
+```pulse
+fn impl_map_group_filter
+  (#t: Type0)
+  (#vmatch2: perm -> t -> cbor & cbor -> slprop)
+  (#cbor_map_iterator_t: Type0)
+  (#cbor_map_iterator_match: perm -> cbor_map_iterator_t -> list (cbor & cbor) -> slprop)
+  (cbor_map_iterator_is_empty: map_iterator_is_empty_t cbor_map_iterator_match)
+  (cbor_map_iterator_next: map_iterator_next_t vmatch2 cbor_map_iterator_match)
+  (#f: Ghost.erased ((cbor & cbor) -> bool))
+  (implf: impl_map_entry_cond vmatch2 f)
+: impl_map_group u#0 #cbor_map_iterator_t cbor_map_iterator_match (map_group_filter f)
+=
+  (i: _)
+  (#p: _)
+  (#l: _)
+  (m: _)
+  (pexcluded: _)
+  (#lexcluded: _)
+  (#vexcluded: _)
+  (_: unit)
+{
+  let mut pi = i;
+  let mut pres = true;
+  let pl1 : GR.ref (list (cbor & cbor)) = GR.alloc (Nil #(cbor & cbor));
+  let mut pj = 0uL;
+  let ll = !pexcluded;
+  Trade.refl (cbor_map_iterator_match p i l);
+  cbor_map_filter_filter f (list_not_defined_at vexcluded) m;
+  list_nil_forall_not_memP (List.Tot.filter (U.andp (list_not_defined_at vexcluded) f) l);
+  Classical.forall_intro_2 (U.list_assoc_no_repeats_mem l);
+  assert (pure (
+    cbor_map_filter f (cbor_map_filter (list_not_defined_at vexcluded) m) `cbor_map_equal'` cbor_map_empty <==> Nil? (List.Tot.filter (U.andp (list_not_defined_at vexcluded) f) l)
+  ));
+  while (
+    let res = !pres;
+    if (res) {
+      with i2 l2 . assert (cbor_map_iterator_match p i2 l2);
+      let j2 = !pi;
+      Trade.rewrite_with_trade
+        (cbor_map_iterator_match p i2 l2)
+        (cbor_map_iterator_match p j2 l2);
+      let is_emp = cbor_map_iterator_is_empty j2;
+      Trade.elim _ (cbor_map_iterator_match p i2 l2);
+      not is_emp
+    } else {
+      false
+    }
+  )
+  invariant b. exists* i2 j l1 l2 res .
+    R.pts_to pi i2 **
+    cbor_map_iterator_match p i2 l2 **
+    R.pts_to pj j **
+    R.pts_to pres res **
+    GR.pts_to pl1 l1 **
+     Trade.trade
+      (cbor_map_iterator_match p i2 l2)
+      (cbor_map_iterator_match p i l) **
+    match_linked_list l ll vexcluded **
+    pure (
+      l == List.Tot.append l1 l2 /\
+      List.Tot.length l1 == U64.v j /\
+      b == (res && Cons? l2) /\
+      (cbor_map_filter f (cbor_map_filter (list_not_defined_at vexcluded) m) == cbor_map_empty <==> (res == true /\ Nil? (List.Tot.filter (U.andp (list_not_defined_at vexcluded) f) l2)))
+    )
+  {
+    let j = !pj;
+    with l1 . assert (GR.pts_to pl1 l1);
+    with gi2 l2 . assert (cbor_map_iterator_match p gi2 l2);
+    list_index_append_cons l1 (List.Tot.hd l2) (List.Tot.tl l2);
+    let entry = cbor_map_iterator_next pi;
+    Trade.trans _ _ (cbor_map_iterator_match p i l);
+    let is_excluded = match_linked_list_mem ll j;
+    pj := U64.add j 1uL;
+    List.Tot.append_assoc l1 [List.Tot.hd l2] (List.Tot.tl l2);
+    List.Tot.append_length l1 [List.Tot.hd l2];
+    GR.op_Colon_Equals pl1 (List.Tot.append l1 [List.Tot.hd l2]);
+    if (not is_excluded) {
+      let matches = implf entry;
+      Trade.elim_hyp_l _ _ _;
+      pres := not matches;
+    } else {
+      Trade.elim_hyp_l _ _ _;
+    }
+  };
+  Trade.elim _ _;
+  GR.free pl1;
+  let res = !pres;
+  if (res) {
+    MGOK
+  } else {
+    MGFail
+  }
+}
+```
+
+inline_for_extraction noextract [@@noextract_to "krml"]
+```pulse
+fn impl_map_group_of_cps
+  (#t: Type0)
+  (#vmatch2: perm -> t -> cbor & cbor -> slprop)
+  (#cbor_map_iterator_t: Type0)
+  (#cbor_map_iterator_match: perm -> cbor_map_iterator_t -> list (cbor & cbor) -> slprop)
+  (cbor_map_iterator_is_empty: map_iterator_is_empty_t cbor_map_iterator_match)
+  (cbor_map_iterator_next: map_iterator_next_t vmatch2 cbor_map_iterator_match)
+  (#g1: Ghost.erased map_group)
+  (ig1: impl_map_group_cps cbor_map_iterator_match g1)
+: impl_map_group u#0 #cbor_map_iterator_t cbor_map_iterator_match g1
+=
+  (i: _)
+  (#p: _)
+  (#l: _)
+  (m: _)
+  (pexcluded: _)
+  (#lexcluded: _)
+  (#vexcluded: _)
+  (_: unit)
+{
+  map_group_concat_nop_r g1;
+  impl_map_group_concat ig1 (impl_map_group_filter cbor_map_iterator_is_empty cbor_map_iterator_next (impl_map_entry_cond_true _)) i #p #l m pexcluded #lexcluded #vexcluded ()
 }
 ```
 
